WIP

code/experimental/SPARKLE/dist/Hacl_Impl_Sparkle.c
@@ -36,18 +36,43 @@ Hacl_Impl_Sparkle_rcon[8U] =
     (uint32_t)0xBB1185EBU, (uint32_t)0x4F7C7B57U, (uint32_t)0xCFBFA1C8U, (uint32_t)0xC2B3293DU
   };
 
-typedef struct branch1_s
+void
+Hacl_Impl_Sparkle_xor_step(uint32_t l, uint32_t *b, uint32_t *tx, uint32_t *ty, uint32_t i)
 {
-  uint32_t fst;
-  uint32_t snd;
+  uint32_t xi = b[(uint32_t)2U * i];
+  uint32_t yi = b[(uint32_t)2U * i + (uint32_t)1U];
+  uint32_t tx_0 = tx[0U];
+  uint32_t ty_0 = ty[0U];
+  tx[0U] = xi ^ tx_0;
+  ty[0U] = yi ^ ty_0;
 }
-branch1;
 
-#include <stdlib.h>
-#include <stdio.h>
-#include <immintrin.h>
-#include <x86intrin.h>
+Spec_SPARKLE2_branch1 Hacl_Impl_Sparkle_xor(uint32_t l, uint32_t *b)
+{
+  uint32_t tx = (uint32_t)0U;
+  uint32_t ty = (uint32_t)0U;
+  for (uint32_t i = (uint32_t)0U; i < l >> (uint32_t)1U; i++)
+  {
+    Hacl_Impl_Sparkle_xor_step(l, b, &tx, &ty, i);
+  }
+  uint32_t r0 = tx;
+  uint32_t r1 = ty;
+  return ((Spec_SPARKLE2_branch1){ .fst = r0, .snd = r1 });
+}
 
+Spec_SPARKLE2_branch1 Hacl_Impl_Sparkle_m(uint32_t n, uint32_t *b)
+{
+  Spec_SPARKLE2_branch1 scrut = Hacl_Impl_Sparkle_xor(n, b);
+  uint32_t ltx = scrut.fst;
+  uint32_t lty = scrut.snd;
+  return
+    (
+      (Spec_SPARKLE2_branch1){
+        .fst = (ltx << (uint32_t)16U | ltx >> (uint32_t)16U) ^ (ltx & (uint32_t)0xffffU),
+        .snd = (lty << (uint32_t)16U | lty >> (uint32_t)16U) ^ (lty & (uint32_t)0xffffU)
+      }
+    );
+}
 
 void Hacl_Impl_Sparkle_l_step(uint32_t n, uint32_t *perm, uint32_t i, uint32_t *result)
 {
@@ -55,7 +80,7 @@ void Hacl_Impl_Sparkle_l_step(uint32_t n, uint32_t *perm, uint32_t i, uint32_t *
   uint32_t yi = result[(uint32_t)2U * i + (uint32_t)1U];
   uint32_t p0i = perm[(uint32_t)2U * i];
   uint32_t p1i = perm[(uint32_t)2U * i + (uint32_t)1U];
-  branch1 branchIUpd = { .fst = xi ^ p0i, .snd = yi ^ p1i };
+  Spec_SPARKLE2_branch1 branchIUpd = { .fst = xi ^ p0i, .snd = yi ^ p1i };
   uint32_t x = branchIUpd.fst;
   uint32_t y = branchIUpd.snd;
   perm[(uint32_t)2U * i] = x;
@@ -64,23 +89,24 @@ void Hacl_Impl_Sparkle_l_step(uint32_t n, uint32_t *perm, uint32_t i, uint32_t *
 
 void Hacl_Impl_Sparkle_arx_n_step(uint32_t n, uint32_t i, uint32_t *b)
 {
-  branch1 branchI = { .fst = b[(uint32_t)2U * i], .snd = b[(uint32_t)2U * i + (uint32_t)1U] };
+  Spec_SPARKLE2_branch1
+  branchI = { .fst = b[(uint32_t)2U * i], .snd = b[(uint32_t)2U * i + (uint32_t)1U] };
   uint32_t rcon_i = Hacl_Impl_Sparkle_rcon[i];
   uint32_t x0 = branchI.fst;
   uint32_t y0 = branchI.snd;
-  uint32_t x1 = x0 + _rotr(y0, 31); 
-  uint32_t y1 = y0 ^ _rotr(x1, 24);
+  uint32_t x1 = x0 + (y0 >> (uint32_t)31U | y0 << (uint32_t)1U);
+  uint32_t y1 = y0 ^ (x1 >> (uint32_t)24U | x1 << (uint32_t)8U);
   uint32_t x2 = x1 ^ rcon_i;
-  uint32_t x3 = x2 + _rotr(y1, 17);
-  uint32_t y2 = y1 ^ _rotr(x3, 17);
+  uint32_t x3 = x2 + (y1 >> (uint32_t)17U | y1 << (uint32_t)15U);
+  uint32_t y2 = y1 ^ (x3 >> (uint32_t)17U | x3 << (uint32_t)15U);
   uint32_t x4 = x3 ^ rcon_i;
   uint32_t x5 = x4 + y2;
-  uint32_t y3 = y2 ^ _rotr(x5, 31);
+  uint32_t y3 = y2 ^ (x5 >> (uint32_t)31U | x5 << (uint32_t)1U);
   uint32_t x6 = x5 ^ rcon_i;
-  uint32_t x7 = x6 + _rotr(y3, 24);
-  uint32_t y4 = y3 ^ _rotr(x7, 16);
+  uint32_t x7 = x6 + (y3 >> (uint32_t)24U | y3 << (uint32_t)8U);
+  uint32_t y4 = y3 ^ (x7 >> (uint32_t)16U | x7 << (uint32_t)16U);
   uint32_t x8 = x7 ^ rcon_i;
-  branch1 scrut = { .fst = x8, .snd = y4 };
+  Spec_SPARKLE2_branch1 scrut = { .fst = x8, .snd = y4 };
   uint32_t x = scrut.fst;
   uint32_t y = scrut.snd;
   b[(uint32_t)2U * i] = x;
@@ -89,78 +115,23 @@ void Hacl_Impl_Sparkle_arx_n_step(uint32_t n, uint32_t i, uint32_t *b)
 
 typedef struct __Spec_SPARKLE2_branch1_Spec_SPARKLE2_branch1_Spec_SPARKLE2_branch1_s
 {
-  branch1 fst;
-  branch1 snd;
-  branch1 thd;
+  Spec_SPARKLE2_branch1 fst;
+  Spec_SPARKLE2_branch1 snd;
+  Spec_SPARKLE2_branch1 thd;
 }
 __Spec_SPARKLE2_branch1_Spec_SPARKLE2_branch1_Spec_SPARKLE2_branch1;
 
 void Hacl_Impl_Sparkle_sparkle256(uint32_t steps, uint8_t *i, uint8_t *o)
 {
   uint32_t temp[12U] = { 0U };
+  for (uint32_t i0 = (uint32_t)0U; i0 < (uint32_t)8U; i0++)
   {
     uint32_t *os = temp;
-    uint8_t *bj = i + (uint32_t)0U * (uint32_t)4U;
+    uint8_t *bj = i + i0 * (uint32_t)4U;
     uint32_t u = load32_le(bj);
     uint32_t r = u;
     uint32_t x = r;
-    os[0U] = x;
-  }
-  {
-    uint32_t *os = temp;
-    uint8_t *bj = i + (uint32_t)1U * (uint32_t)4U;
-    uint32_t u = load32_le(bj);
-    uint32_t r = u;
-    uint32_t x = r;
-    os[1U] = x;
-  }
-  {
-    uint32_t *os = temp;
-    uint8_t *bj = i + (uint32_t)2U * (uint32_t)4U;
-    uint32_t u = load32_le(bj);
-    uint32_t r = u;
-    uint32_t x = r;
-    os[2U] = x;
-  }
-  {
-    uint32_t *os = temp;
-    uint8_t *bj = i + (uint32_t)3U * (uint32_t)4U;
-    uint32_t u = load32_le(bj);
-    uint32_t r = u;
-    uint32_t x = r;
-    os[3U] = x;
-  }
-  {
-    uint32_t *os = temp;
-    uint8_t *bj = i + (uint32_t)4U * (uint32_t)4U;
-    uint32_t u = load32_le(bj);
-    uint32_t r = u;
-    uint32_t x = r;
-    os[4U] = x;
-  }
-  {
-    uint32_t *os = temp;
-    uint8_t *bj = i + (uint32_t)5U * (uint32_t)4U;
-    uint32_t u = load32_le(bj);
-    uint32_t r = u;
-    uint32_t x = r;
-    os[5U] = x;
-  }
-  {
-    uint32_t *os = temp;
-    uint8_t *bj = i + (uint32_t)6U * (uint32_t)4U;
-    uint32_t u = load32_le(bj);
-    uint32_t r = u;
-    uint32_t x = r;
-    os[6U] = x;
-  }
-  {
-    uint32_t *os = temp;
-    uint8_t *bj = i + (uint32_t)7U * (uint32_t)4U;
-    uint32_t u = load32_le(bj);
-    uint32_t r = u;
-    uint32_t x = r;
-    os[7U] = x;
+    os[i0] = x;
   }
   for (uint32_t i1 = (uint32_t)0U; i1 < steps; i1++)
   {
@@ -187,31 +158,7 @@ void Hacl_Impl_Sparkle_sparkle256(uint32_t steps, uint8_t *i, uint8_t *o)
     {
       Hacl_Impl_Sparkle_arx_n_step((uint32_t)4U, (uint32_t)3U, temp);
     }
-    uint32_t tx = (uint32_t)0U;
-    uint32_t ty = (uint32_t)0U;
-    {
-      uint32_t xi = temp[(uint32_t)2U * (uint32_t)0U];
-      uint32_t yi = temp[(uint32_t)2U * (uint32_t)0U + (uint32_t)1U];
-      uint32_t tx_0 = tx;
-      uint32_t ty_0 = ty;
-      tx = xi ^ tx_0;
-      ty = yi ^ ty_0;
-    }
-    {
-      uint32_t xi = temp[(uint32_t)2U * (uint32_t)1U];
-      uint32_t yi = temp[(uint32_t)2U * (uint32_t)1U + (uint32_t)1U];
-      uint32_t tx_0 = tx;
-      uint32_t ty_0 = ty;
-      tx = xi ^ tx_0;
-      ty = yi ^ ty_0;
-    }
-    uint32_t uu____0 = tx;
-    uint32_t
-    ltx0 = (uu____0 << (uint32_t)16U | uu____0 >> (uint32_t)16U) ^ (uu____0 & (uint32_t)0xffffU);
-    uint32_t uu____1 = ty;
-    uint32_t
-    lty0 = (uu____1 << (uint32_t)16U | uu____1 >> (uint32_t)16U) ^ (uu____1 & (uint32_t)0xffffU);
-    branch1 scrut = { .fst = ltx0, .snd = lty0 };
+    Spec_SPARKLE2_branch1 scrut = Hacl_Impl_Sparkle_m((uint32_t)4U, temp);
     uint32_t ltx = scrut.fst;
     uint32_t lty = scrut.snd;
     uint32_t x0 = (uint32_t)0U;
@@ -219,13 +166,13 @@ void Hacl_Impl_Sparkle_sparkle256(uint32_t steps, uint8_t *i, uint8_t *o)
     x0 = temp[0U];
     y0 = temp[1U];
     {
-      branch1
+      Spec_SPARKLE2_branch1
       branch_j_nb =
         {
           .fst = temp[(uint32_t)2U * ((uint32_t)0U + (uint32_t)1U + (uint32_t)2U)],
           .snd = temp[(uint32_t)2U * ((uint32_t)0U + (uint32_t)1U + (uint32_t)2U) + (uint32_t)1U]
         };
-      branch1
+      Spec_SPARKLE2_branch1
       branch_j =
         {
           .fst = temp[(uint32_t)2U * ((uint32_t)0U + (uint32_t)1U)],
@@ -241,7 +188,7 @@ void Hacl_Impl_Sparkle_sparkle256(uint32_t steps, uint8_t *i, uint8_t *o)
       uint32_t i0x = scrut0.fst.fst;
       uint32_t o0_x = i0x ^ (i1x ^ i2x);
       uint32_t o0_y = i0y ^ (i1y ^ i2y);
-      branch1 b0 = { .fst = o0_x, .snd = o0_y };
+      Spec_SPARKLE2_branch1 b0 = { .fst = o0_x, .snd = o0_y };
       uint32_t x = b0.fst;
       uint32_t y2 = b0.snd;
       temp[(uint32_t)2U * (uint32_t)0U] = x;
@@ -261,7 +208,7 @@ void Hacl_Impl_Sparkle_sparkle256(uint32_t steps, uint8_t *i, uint8_t *o)
     uint32_t i2y = ltx;
     uint32_t o0_x = i0x ^ (i1x ^ i2x);
     uint32_t o0_y = i0y ^ (i1y ^ i2y);
-    branch1 last0 = { .fst = o0_x, .snd = o0_y };
+    Spec_SPARKLE2_branch1 last0 = { .fst = o0_x, .snd = o0_y };
     uint32_t x = last0.fst;
     uint32_t y = last0.snd;
     temp[(uint32_t)2U * ((uint32_t)2U - (uint32_t)1U)] = x;
@@ -269,29 +216,9 @@ void Hacl_Impl_Sparkle_sparkle256(uint32_t steps, uint8_t *i, uint8_t *o)
     temp[4U] = x01;
     temp[5U] = y01;
   }
+  for (uint32_t i0 = (uint32_t)0U; i0 < (uint32_t)8U; i0++)
   {
-    store32_le(o + (uint32_t)0U * (uint32_t)4U, temp[0U]);
-  }
-  {
-    store32_le(o + (uint32_t)1U * (uint32_t)4U, temp[1U]);
-  }
-  {
-    store32_le(o + (uint32_t)2U * (uint32_t)4U, temp[2U]);
-  }
-  {
-    store32_le(o + (uint32_t)3U * (uint32_t)4U, temp[3U]);
-  }
-  {
-    store32_le(o + (uint32_t)4U * (uint32_t)4U, temp[4U]);
-  }
-  {
-    store32_le(o + (uint32_t)5U * (uint32_t)4U, temp[5U]);
-  }
-  {
-    store32_le(o + (uint32_t)6U * (uint32_t)4U, temp[6U]);
-  }
-  {
-    store32_le(o + (uint32_t)7U * (uint32_t)4U, temp[7U]);
+    store32_le(o + i0 * (uint32_t)4U, temp[i0]);
   }
 }
 
