code/experimental/SPARKLE/dist/Hacl_Impl_Sparkle1.c
@@ -1,0 +1,259 @@
+/* MIT License
+ *
+ * Copyright (c) 2016-2020 INRIA, CMU and Microsoft Corporation
+ *
+ * Permission is hereby granted, free of charge, to any person obtaining a copy
+ * of this software and associated documentation files (the "Software"), to deal
+ * in the Software without restriction, including without limitation the rights
+ * to use, copy, modify, merge, publish, distribute, sublicense, and/or sell
+ * copies of the Software, and to permit persons to whom the Software is
+ * furnished to do so, subject to the following conditions:
+ *
+ * The above copyright notice and this permission notice shall be included in all
+ * copies or substantial portions of the Software.
+ *
+ * THE SOFTWARE IS PROVIDED "AS IS", WITHOUT WARRANTY OF ANY KIND, EXPRESS OR
+ * IMPLIED, INCLUDING BUT NOT LIMITED TO THE WARRANTIES OF MERCHANTABILITY,
+ * FITNESS FOR A PARTICULAR PURPOSE AND NONINFRINGEMENT. IN NO EVENT SHALL THE
+ * AUTHORS OR COPYRIGHT HOLDERS BE LIABLE FOR ANY CLAIM, DAMAGES OR OTHER
+ * LIABILITY, WHETHER IN AN ACTION OF CONTRACT, TORT OR OTHERWISE, ARISING FROM,
+ * OUT OF OR IN CONNECTION WITH THE SOFTWARE OR THE USE OR OTHER DEALINGS IN THE
+ * SOFTWARE.
+ */
+
+
+#include "Hacl_Impl_Sparkle1.h"
+
+uint32_t Hacl_Impl_Sparkle1_vsize_rcon = (uint32_t)8U;
+
+const
+uint32_t
+Hacl_Impl_Sparkle1_rcon[8U] =
+  {
+    (uint32_t)0xB7E15162U, (uint32_t)0xBF715880U, (uint32_t)0x38B4DA56U, (uint32_t)0x324E7738U,
+    (uint32_t)0xBB1185EBU, (uint32_t)0x4F7C7B57U, (uint32_t)0xCFBFA1C8U, (uint32_t)0xC2B3293DU
+  };
+
+Spec_SPARKLE2_branch1 Hacl_Impl_Sparkle1_xor(uint32_t l, uint32_t *b)
+{
+  uint32_t tx = (uint32_t)0U;
+  uint32_t ty = (uint32_t)0U;
+  for (uint32_t i = (uint32_t)0U; i < l >> (uint32_t)1U; i++)
+  {
+    uint32_t xi = b[(uint32_t)2U * i];
+    uint32_t yi = b[(uint32_t)2U * i + (uint32_t)1U];
+    uint32_t tx_0 = tx;
+    uint32_t ty_0 = ty;
+    tx = xi ^ tx_0;
+    ty = yi ^ ty_0;
+  }
+  uint32_t r0 = tx;
+  uint32_t r1 = ty;
+  return ((Spec_SPARKLE2_branch1){ .fst = r0, .snd = r1 });
+}
+
+void
+Hacl_Impl_Sparkle1_xor_x(uint32_t n, uint32_t *b, uint32_t lty, uint32_t ltx, uint32_t *temp)
+{
+  for (uint32_t i = (uint32_t)0U; i < n >> (uint32_t)1U; i++)
+  {
+    uint32_t xi = b[(uint32_t)2U * i];
+    uint32_t yi = b[(uint32_t)2U * i + (uint32_t)1U];
+    uint32_t xi_n = xi ^ lty;
+    uint32_t yi_n = yi ^ ltx;
+    temp[(uint32_t)2U * i] = xi_n;
+    temp[(uint32_t)2U * i + (uint32_t)1U] = yi_n;
+  }
+}
+
+void Hacl_Impl_Sparkle1_l_step(uint32_t n, uint32_t *m1, uint32_t i, uint32_t *right)
+{
+  uint32_t xi = right[(uint32_t)2U * i];
+  uint32_t yi = right[(uint32_t)2U * i + (uint32_t)1U];
+  uint32_t p0i = m1[(uint32_t)2U * i];
+  uint32_t p1i = m1[(uint32_t)2U * i + (uint32_t)1U];
+  Spec_SPARKLE2_branch1 branchIUpd = { .fst = xi ^ p0i, .snd = yi ^ p1i };
+  uint32_t x = branchIUpd.fst;
+  uint32_t y = branchIUpd.snd;
+  m1[(uint32_t)2U * i] = x;
+  m1[(uint32_t)2U * i + (uint32_t)1U] = y;
+}
+
+void Hacl_Impl_Sparkle1_l(uint32_t n, uint32_t *b)
+{
+  KRML_CHECK_SIZE(sizeof (uint32_t), (uint32_t)2U * n);
+  uint32_t result[(uint32_t)2U * n];
+  memset(result, 0U, (uint32_t)2U * n * sizeof (uint32_t));
+  uint32_t *leftBranch = b;
+  uint32_t *rightBranch = b + n;
+  uint32_t tx = (uint32_t)0U;
+  uint32_t ty = (uint32_t)0U;
+  for (uint32_t i = (uint32_t)0U; i < n >> (uint32_t)1U; i++)
+  {
+    uint32_t xi = b[(uint32_t)2U * i];
+    uint32_t yi = b[(uint32_t)2U * i + (uint32_t)1U];
+    uint32_t tx_0 = tx;
+    uint32_t ty_0 = ty;
+    tx = xi ^ tx_0;
+    ty = yi ^ ty_0;
+  }
+  uint32_t r0 = tx;
+  uint32_t r1 = ty;
+  Spec_SPARKLE2_branch1 scrut = { .fst = r0, .snd = r1 };
+  uint32_t ltx = scrut.fst;
+  uint32_t lty = scrut.snd;
+  Hacl_Impl_Sparkle1_xor_x(n,
+    b,
+    (lty << (uint32_t)16U | lty >> (uint32_t)16U) ^ (lty & (uint32_t)0xffffU),
+    (ltx << (uint32_t)16U | ltx >> (uint32_t)16U) ^ (ltx & (uint32_t)0xffffU),
+    result);
+  for (uint32_t i = (uint32_t)0U; i < n >> (uint32_t)1U; i++)
+  {
+    uint32_t xi = rightBranch[(uint32_t)2U * i];
+    uint32_t yi = rightBranch[(uint32_t)2U * i + (uint32_t)1U];
+    uint32_t p0i = result[(uint32_t)2U * i];
+    uint32_t p1i = result[(uint32_t)2U * i + (uint32_t)1U];
+    Spec_SPARKLE2_branch1 branchIUpd = { .fst = xi ^ p0i, .snd = yi ^ p1i };
+    uint32_t x = branchIUpd.fst;
+    uint32_t y = branchIUpd.snd;
+    result[(uint32_t)2U * i] = x;
+    result[(uint32_t)2U * i + (uint32_t)1U] = y;
+  }
+  for (uint32_t i = (uint32_t)0U; i < n >> (uint32_t)1U; i++)
+  {
+    uint32_t x = leftBranch[(uint32_t)2U * i];
+    uint32_t y = leftBranch[(uint32_t)2U * i + (uint32_t)1U];
+    rightBranch[(uint32_t)2U * i] = x;
+    rightBranch[(uint32_t)2U * i + (uint32_t)1U] = y;
+  }
+  for (uint32_t i = (uint32_t)0U; i < n >> (uint32_t)1U; i++)
+  {
+    uint32_t index = i - (uint32_t)1U;
+    uint32_t k = n >> (uint32_t)1U;
+    uint32_t j = index % k;
+    uint32_t x = result[(uint32_t)2U * i];
+    uint32_t y = result[(uint32_t)2U * i + (uint32_t)1U];
+    leftBranch[(uint32_t)2U * j] = x;
+    leftBranch[(uint32_t)2U * j + (uint32_t)1U] = y;
+  }
+}
+
+void Hacl_Impl_Sparkle1_add2(uint32_t n, uint32_t i, uint32_t *b)
+{
+  uint32_t x0 = b[0U];
+  uint32_t y0 = b[1U];
+  uint32_t x1 = b[2U];
+  uint32_t y1 = b[3U];
+  uint32_t i0 = i & (uint32_t)7U;
+  uint32_t y01 = y0 ^ Hacl_Impl_Sparkle1_rcon[i0];
+  uint32_t y11 = y1 ^ i;
+  b[0U] = x0;
+  b[1U] = y01;
+  b[2U] = x1;
+  b[3U] = y11;
+}
+
+void Hacl_Impl_Sparkle1_toBranch(uint32_t n, uint8_t *i, uint32_t *o)
+{
+  for (uint32_t i0 = (uint32_t)0U; i0 < (uint32_t)2U * n; i0++)
+  {
+    uint32_t *os = o;
+    uint8_t *bj = i + i0 * (uint32_t)4U;
+    uint32_t u = load32_le(bj);
+    uint32_t r = u;
+    uint32_t x = r;
+    os[i0] = x;
+  }
+}
+
+void Hacl_Impl_Sparkle1_fromBranch(uint32_t n, uint32_t *i, uint8_t *o)
+{
+  for (uint32_t i0 = (uint32_t)0U; i0 < (uint32_t)2U * n; i0++)
+  {
+    store32_le(o + i0 * (uint32_t)4U, i[i0]);
+  }
+}
+
+void Hacl_Impl_Sparkle1_arx_n_step(uint32_t n, uint32_t i, uint32_t *b)
+{
+  Spec_SPARKLE2_branch1
+  branchI = { .fst = b[(uint32_t)2U * i], .snd = b[(uint32_t)2U * i + (uint32_t)1U] };
+  uint32_t rcon_i = Hacl_Impl_Sparkle1_rcon[i];
+  uint32_t x0 = branchI.fst;
+  uint32_t y0 = branchI.snd;
+  uint32_t x1 = x0 + (y0 >> (uint32_t)31U | y0 << (uint32_t)1U);
+  uint32_t y1 = y0 ^ (x1 >> (uint32_t)24U | x1 << (uint32_t)8U);
+  uint32_t x2 = x1 ^ rcon_i;
+  uint32_t x3 = x2 + (y1 >> (uint32_t)17U | y1 << (uint32_t)15U);
+  uint32_t y2 = y1 ^ (x3 >> (uint32_t)17U | x3 << (uint32_t)15U);
+  uint32_t x4 = x3 ^ rcon_i;
+  uint32_t x5 = x4 + y2;
+  uint32_t y3 = y2 ^ (x5 >> (uint32_t)31U | x5 << (uint32_t)1U);
+  uint32_t x6 = x5 ^ rcon_i;
+  uint32_t x7 = x6 + (y3 >> (uint32_t)24U | y3 << (uint32_t)8U);
+  uint32_t y4 = y3 ^ (x7 >> (uint32_t)16U | x7 << (uint32_t)16U);
+  uint32_t x8 = x7 ^ rcon_i;
+  Spec_SPARKLE2_branch1 scrut = { .fst = x8, .snd = y4 };
+  uint32_t x = scrut.fst;
+  uint32_t y = scrut.snd;
+  b[(uint32_t)2U * i] = x;
+  b[(uint32_t)2U * i + (uint32_t)1U] = y;
+}
+
+void Hacl_Impl_Sparkle1_sparkle256(uint32_t steps, uint8_t *i, uint8_t *o)
+{
+  uint32_t len = (uint32_t)4U;
+  KRML_CHECK_SIZE(sizeof (uint32_t), len * (uint32_t)2U);
+  uint32_t temp[len * (uint32_t)2U];
+  memset(temp, 0U, len * (uint32_t)2U * sizeof (uint32_t));
+  Hacl_Impl_Sparkle1_toBranch(len, i, temp);
+  for (uint32_t i0 = (uint32_t)0U; i0 < steps; i0++)
+  {
+    Hacl_Impl_Sparkle1_add2(len, i0, temp);
+    for (uint32_t i1 = (uint32_t)0U; i1 < len; i1++)
+    {
+      Hacl_Impl_Sparkle1_arx_n_step(len, i1, temp);
+    }
+    Hacl_Impl_Sparkle1_l(len, temp);
+  }
+  Hacl_Impl_Sparkle1_fromBranch(len, temp, o);
+}
+
+void Hacl_Impl_Sparkle1_sparkle384(uint32_t steps, uint8_t *i, uint8_t *o)
+{
+  uint32_t len = (uint32_t)6U;
+  KRML_CHECK_SIZE(sizeof (uint32_t), len * (uint32_t)2U);
+  uint32_t temp[len * (uint32_t)2U];
+  memset(temp, 0U, len * (uint32_t)2U * sizeof (uint32_t));
+  Hacl_Impl_Sparkle1_toBranch(len, i, temp);
+  for (uint32_t i0 = (uint32_t)0U; i0 < steps; i0++)
+  {
+    Hacl_Impl_Sparkle1_add2(len, i0, temp);
+    for (uint32_t i1 = (uint32_t)0U; i1 < len; i1++)
+    {
+      Hacl_Impl_Sparkle1_arx_n_step(len, i1, temp);
+    }
+    Hacl_Impl_Sparkle1_l(len, temp);
+  }
+  Hacl_Impl_Sparkle1_fromBranch(len, temp, o);
+}
+
+void Hacl_Impl_Sparkle1_sparkle512(uint32_t steps, uint8_t *i, uint8_t *o)
+{
+  uint32_t len = (uint32_t)8U;
+  KRML_CHECK_SIZE(sizeof (uint32_t), len * (uint32_t)2U);
+  uint32_t temp[len * (uint32_t)2U];
+  memset(temp, 0U, len * (uint32_t)2U * sizeof (uint32_t));
+  Hacl_Impl_Sparkle1_toBranch(len, i, temp);
+  for (uint32_t i0 = (uint32_t)0U; i0 < steps; i0++)
+  {
+    Hacl_Impl_Sparkle1_add2(len, i0, temp);
+    for (uint32_t i1 = (uint32_t)0U; i1 < len; i1++)
+    {
+      Hacl_Impl_Sparkle1_arx_n_step(len, i1, temp);
+    }
+    Hacl_Impl_Sparkle1_l(len, temp);
+  }
+  Hacl_Impl_Sparkle1_fromBranch(len, temp, o);
+}
+
